\documentclass[10pt]{amsart}

%Packages in use
\usepackage{fullpage, hyperref, vipul, enumerate}

%Title details
\title{Class quiz: March 4: Series convergence}
\author{Math 153, Section 55 (Vipul Naik)}
%List of new commands

\begin{document}
\maketitle

Your name (print clearly in capital letters): $\underline{\qquad\qquad\qquad\qquad\qquad\qquad\qquad\qquad\qquad\qquad}$

\begin{enumerate}


\item Consider the function $f(x) := \sum_{n=1}^\infty
  \frac{x^n}{n(n + 2)}$ defined on the closed interval
  $[-1,1]$. What are the values of $f(1)$ and $f(-1)$?

  \begin{enumerate}[(A)]
  \item $f(1) = 3/4$ and $f(-1) = 1/4$
  \item $f(1) = 3/4$ and $f(-1) = -1/4$
  \item $f(1) = 3/4$ and $f(-1) = -3/4$
  \item $f(1) = 1/4$ and $f(-1) = 3/4$
  \item $f(1) = 1/4$ and $f(-1) = -1/4$
  \end{enumerate}

  \vspace{0.1in}
  Your answer: $\underline{\qquad\qquad\qquad\qquad\qquad\qquad\qquad}$
  \vspace{0.15in}

\item Given that we have the following: $\sum_{n=1}^\infty x^n/n =
  -\ln(1 - x)$ for all $-1 < x < 1$ and the series converges
  absolutely in the interval, what is an explicit expression for the
  summation $\sum_{n=1}^\infty x^n/(n(n+1))$ for $x \in (-1,1)
  \setminus \{ 0 \}$?

  \begin{enumerate}[(A)]
  \item $1 + \ln(1 - x)$
  \item $1 - \ln(1 - x)$
  \item $1 + \frac{(1 + x)\ln(1 - x)}{x}$
  \item $1 + \frac{(1 - x)\ln(1 - x)}{x}$
  \item $1 + \frac{(x - 1)\ln(1 - x)}{x}$
  \end{enumerate}

  \vspace{0.1in}
  Your answer: $\underline{\qquad\qquad\qquad\qquad\qquad\qquad\qquad}$
  \vspace{0.15in}

\item Given that we have the following: $\sum_{n=1}^\infty x^n/n =
  -\ln(1 - x)$ for all $-1 < x < 1$ and the series converges
  absolutely in the interval, what is an explicit expression for the
  summation $\sum_{n=1}^\infty x^n/(n(n+2))$ for $x \in (-1,1)
  \setminus \{ 0 \}$?

  \begin{enumerate}[(A)]
  \item $\frac{1}{4} + \frac{1}{2x} + \frac{(1 - x^2)\ln(1 - x)}{2x^2}$
  \item $\frac{1}{4} + \frac{1}{2x} + \frac{(x^2 - 1)\ln(1 - x)}{2x^2}$
  \item $\frac{1}{4} - \frac{1}{2x} + \frac{(x^2 - 1)\ln(1 - x)}{2x^2}$
  \item $\frac{1}{4} - \frac{1}{2x} + \frac{(1 - x^2)\ln(1 - x)}{2x^2}$
  \item $\frac{1}{4} + \frac{1}{2x}$
  \end{enumerate}

  \vspace{0.1in}
  Your answer: $\underline{\qquad\qquad\qquad\qquad\qquad\qquad\qquad}$
  \vspace{0.15in}

\end{enumerate}

\end{document}
